HOL/DataStrs/Arrays_Ex.thy
@@ -25,6 +25,9 @@ setup {* add_forward_prfstep_cond @{thm length_list_swap} [with_term "list_swap 
 
 lemma mset_list_swap [rewrite]:
   "i < length xs \<Longrightarrow> j < length xs \<Longrightarrow> mset (list_swap xs i j) = mset xs" by auto2
+
+lemma set_list_swap [rewrite]:
+  "i < length xs \<Longrightarrow> j < length xs \<Longrightarrow> set (list_swap xs i j) = set xs" by auto2
 setup {* del_prfstep_thm @{thm list_swap_def} *}
 setup {* add_rewrite_rule_back @{thm list_swap_def} *}
 
